Fixing proofs

Cpc/Proofs/TypePreservation/Support.lean
@@ -18,9 +18,9 @@ inductive supported_preservation_term : SmtTerm -> Prop
   | uconst (s : native_String) (T : SmtType)
       (hT : type_inhabited T) :
       supported_preservation_term (SmtTerm.UConst s T)
-  | re_allchar : supported_preservation_term SmtTerm.re_allchar
-  | re_none : supported_preservation_term SmtTerm.re_none
-  | re_all : supported_preservation_term SmtTerm.re_all
+  | re_allchar : supported_preservation_term (SmtTerm.TheoryOp SmtTheoryOp.re_allchar)
+  | re_none : supported_preservation_term (SmtTerm.TheoryOp SmtTheoryOp.re_none)
+  | re_all : supported_preservation_term (SmtTerm.TheoryOp SmtTheoryOp.re_all)
   | seq_empty (T : SmtType)
       (hT : type_inhabited T) :
       supported_preservation_term (SmtTerm.seq_empty T)
@@ -30,55 +30,55 @@ inductive supported_preservation_term : SmtTerm -> Prop
   | seq_unit {t : SmtTerm}
       (ht : term_has_non_none_type t)
       (hs : supported_preservation_term t) :
-      supported_preservation_term (SmtTerm.seq_unit t)
+      supported_preservation_term (theory1 SmtTheoryOp.seq_unit t)
   | set_singleton {t : SmtTerm}
       (ht : term_has_non_none_type t)
       (hs : supported_preservation_term t) :
-      supported_preservation_term (SmtTerm.set_singleton t)
+      supported_preservation_term (theory1 SmtTheoryOp.set_singleton t)
   | seq_nth {t1 t2 : SmtTerm}
       (ht1 : term_has_non_none_type t1)
       (hs1 : supported_preservation_term t1)
       (ht2 : term_has_non_none_type t2)
       (hs2 : supported_preservation_term t2)
       (hT :
-        type_inhabited (__smtx_typeof (SmtTerm.seq_nth t1 t2))) :
-      supported_preservation_term (SmtTerm.seq_nth t1 t2)
+        type_inhabited (__smtx_typeof (theory2 SmtTheoryOp.seq_nth t1 t2))) :
+      supported_preservation_term (theory2 SmtTheoryOp.seq_nth t1 t2)
   | set_union {t1 t2 : SmtTerm}
       (ht1 : term_has_non_none_type t1)
       (hs1 : supported_preservation_term t1)
       (ht2 : term_has_non_none_type t2)
       (hs2 : supported_preservation_term t2) :
-      supported_preservation_term (SmtTerm.set_union t1 t2)
+      supported_preservation_term (theory2 SmtTheoryOp.set_union t1 t2)
   | set_inter {t1 t2 : SmtTerm}
       (ht1 : term_has_non_none_type t1)
       (hs1 : supported_preservation_term t1)
       (ht2 : term_has_non_none_type t2)
       (hs2 : supported_preservation_term t2) :
-      supported_preservation_term (SmtTerm.set_inter t1 t2)
+      supported_preservation_term (theory2 SmtTheoryOp.set_inter t1 t2)
   | set_minus {t1 t2 : SmtTerm}
       (ht1 : term_has_non_none_type t1)
       (hs1 : supported_preservation_term t1)
       (ht2 : term_has_non_none_type t2)
       (hs2 : supported_preservation_term t2) :
-      supported_preservation_term (SmtTerm.set_minus t1 t2)
+      supported_preservation_term (theory2 SmtTheoryOp.set_minus t1 t2)
   | set_member {t1 t2 : SmtTerm}
       (ht1 : term_has_non_none_type t1)
       (hs1 : supported_preservation_term t1)
       (ht2 : term_has_non_none_type t2)
       (hs2 : supported_preservation_term t2) :
-      supported_preservation_term (SmtTerm.set_member t1 t2)
+      supported_preservation_term (theory2 SmtTheoryOp.set_member t1 t2)
   | set_subset {t1 t2 : SmtTerm}
       (ht1 : term_has_non_none_type t1)
       (hs1 : supported_preservation_term t1)
       (ht2 : term_has_non_none_type t2)
       (hs2 : supported_preservation_term t2) :
-      supported_preservation_term (SmtTerm.set_subset t1 t2)
+      supported_preservation_term (theory2 SmtTheoryOp.set_subset t1 t2)
   | select {t1 t2 : SmtTerm}
       (ht1 : term_has_non_none_type t1)
       (hs1 : supported_preservation_term t1)
       (ht2 : term_has_non_none_type t2)
       (hs2 : supported_preservation_term t2) :
-      supported_preservation_term (SmtTerm.select t1 t2)
+      supported_preservation_term (theory2 SmtTheoryOp.select t1 t2)
   | store {t1 t2 t3 : SmtTerm}
       (ht1 : term_has_non_none_type t1)
       (hs1 : supported_preservation_term t1)
@@ -87,7 +87,7 @@ inductive supported_preservation_term : SmtTerm -> Prop
       (ht3 : term_has_non_none_type t3)
       (hs3 : supported_preservation_term t3) :
       supported_preservation_term
-        (SmtTerm.store t1 t2 t3)
+        (theory3 SmtTheoryOp.store t1 t2 t3)
   | ite {c t1 t2 : SmtTerm}
       (htc : term_has_non_none_type c)
       (hsc : supported_preservation_term c)
@@ -106,171 +106,171 @@ inductive supported_preservation_term : SmtTerm -> Prop
   | not {t : SmtTerm}
       (ht : term_has_non_none_type t)
       (hs : supported_preservation_term t) :
-      supported_preservation_term (SmtTerm.not t)
+      supported_preservation_term (theory1 SmtTheoryOp.not t)
   | or {t1 t2 : SmtTerm}
       (ht1 : term_has_non_none_type t1)
       (hs1 : supported_preservation_term t1)
       (ht2 : term_has_non_none_type t2)
       (hs2 : supported_preservation_term t2) :
-      supported_preservation_term (SmtTerm.or t1 t2)
+      supported_preservation_term (theory2 SmtTheoryOp.or t1 t2)
   | and {t1 t2 : SmtTerm}
       (ht1 : term_has_non_none_type t1)
       (hs1 : supported_preservation_term t1)
       (ht2 : term_has_non_none_type t2)
       (hs2 : supported_preservation_term t2) :
-      supported_preservation_term (SmtTerm.and t1 t2)
+      supported_preservation_term (theory2 SmtTheoryOp.and t1 t2)
   | imp {t1 t2 : SmtTerm}
       (ht1 : term_has_non_none_type t1)
       (hs1 : supported_preservation_term t1)
       (ht2 : term_has_non_none_type t2)
       (hs2 : supported_preservation_term t2) :
-      supported_preservation_term (SmtTerm.imp t1 t2)
+      supported_preservation_term (theory2 SmtTheoryOp.imp t1 t2)
   | eq (t1 t2 : SmtTerm) :
       supported_preservation_term (SmtTerm.eq t1 t2)
   | xor (t1 t2 : SmtTerm) :
-      supported_preservation_term (SmtTerm.xor t1 t2)
+      supported_preservation_term (theory2 SmtTheoryOp.xor t1 t2)
   | plus {t1 t2 : SmtTerm}
       (ht1 : term_has_non_none_type t1)
       (hs1 : supported_preservation_term t1)
       (ht2 : term_has_non_none_type t2)
       (hs2 : supported_preservation_term t2) :
-      supported_preservation_term (SmtTerm.plus t1 t2)
+      supported_preservation_term (theory2 SmtTheoryOp.plus t1 t2)
   | arith_neg {t1 t2 : SmtTerm}
       (ht1 : term_has_non_none_type t1)
       (hs1 : supported_preservation_term t1)
       (ht2 : term_has_non_none_type t2)
       (hs2 : supported_preservation_term t2) :
-      supported_preservation_term (SmtTerm.neg t1 t2)
+      supported_preservation_term (theory2 SmtTheoryOp.neg t1 t2)
   | mult {t1 t2 : SmtTerm}
       (ht1 : term_has_non_none_type t1)
       (hs1 : supported_preservation_term t1)
       (ht2 : term_has_non_none_type t2)
       (hs2 : supported_preservation_term t2) :
-      supported_preservation_term (SmtTerm.mult t1 t2)
+      supported_preservation_term (theory2 SmtTheoryOp.mult t1 t2)
   | lt {t1 t2 : SmtTerm}
       (ht1 : term_has_non_none_type t1)
       (hs1 : supported_preservation_term t1)
       (ht2 : term_has_non_none_type t2)
       (hs2 : supported_preservation_term t2) :
-      supported_preservation_term (SmtTerm.lt t1 t2)
+      supported_preservation_term (theory2 SmtTheoryOp.lt t1 t2)
   | leq {t1 t2 : SmtTerm}
       (ht1 : term_has_non_none_type t1)
       (hs1 : supported_preservation_term t1)
       (ht2 : term_has_non_none_type t2)
       (hs2 : supported_preservation_term t2) :
-      supported_preservation_term (SmtTerm.leq t1 t2)
+      supported_preservation_term (theory2 SmtTheoryOp.leq t1 t2)
   | gt {t1 t2 : SmtTerm}
       (ht1 : term_has_non_none_type t1)
       (hs1 : supported_preservation_term t1)
       (ht2 : term_has_non_none_type t2)
       (hs2 : supported_preservation_term t2) :
-      supported_preservation_term (SmtTerm.gt t1 t2)
+      supported_preservation_term (theory2 SmtTheoryOp.gt t1 t2)
   | geq {t1 t2 : SmtTerm}
       (ht1 : term_has_non_none_type t1)
       (hs1 : supported_preservation_term t1)
       (ht2 : term_has_non_none_type t2)
       (hs2 : supported_preservation_term t2) :
-      supported_preservation_term (SmtTerm.geq t1 t2)
+      supported_preservation_term (theory2 SmtTheoryOp.geq t1 t2)
   | to_real {t : SmtTerm}
       (ht : term_has_non_none_type t)
       (hs : supported_preservation_term t) :
-      supported_preservation_term (SmtTerm.to_real t)
+      supported_preservation_term (theory1 SmtTheoryOp.to_real t)
   | to_int {t : SmtTerm}
       (ht : term_has_non_none_type t)
       (hs : supported_preservation_term t) :
-      supported_preservation_term (SmtTerm.to_int t)
+      supported_preservation_term (theory1 SmtTheoryOp.to_int t)
   | is_int {t : SmtTerm}
       (ht : term_has_non_none_type t)
       (hs : supported_preservation_term t) :
-      supported_preservation_term (SmtTerm.is_int t)
+      supported_preservation_term (theory1 SmtTheoryOp.is_int t)
   | abs {t : SmtTerm}
       (ht : term_has_non_none_type t)
       (hs : supported_preservation_term t) :
-      supported_preservation_term (SmtTerm.abs t)
+      supported_preservation_term (theory1 SmtTheoryOp.abs t)
   | uneg {t : SmtTerm}
       (ht : term_has_non_none_type t)
       (hs : supported_preservation_term t) :
-      supported_preservation_term (SmtTerm.uneg t)
+      supported_preservation_term (theory1 SmtTheoryOp.uneg t)
   | div {t1 t2 : SmtTerm}
       (ht1 : term_has_non_none_type t1)
       (hs1 : supported_preservation_term t1)
       (ht2 : term_has_non_none_type t2)
       (hs2 : supported_preservation_term t2) :
-      supported_preservation_term (SmtTerm.div t1 t2)
+      supported_preservation_term (theory2 SmtTheoryOp.div t1 t2)
   | mod {t1 t2 : SmtTerm}
       (ht1 : term_has_non_none_type t1)
       (hs1 : supported_preservation_term t1)
       (ht2 : term_has_non_none_type t2)
       (hs2 : supported_preservation_term t2) :
-      supported_preservation_term (SmtTerm.mod t1 t2)
+      supported_preservation_term (theory2 SmtTheoryOp.mod t1 t2)
   | multmult {t1 t2 : SmtTerm}
       (ht1 : term_has_non_none_type t1)
       (hs1 : supported_preservation_term t1)
       (ht2 : term_has_non_none_type t2)
       (hs2 : supported_preservation_term t2) :
-      supported_preservation_term (SmtTerm.multmult t1 t2)
+      supported_preservation_term (theory2 SmtTheoryOp.multmult t1 t2)
   | divisible {t1 t2 : SmtTerm}
       (ht1 : term_has_non_none_type t1)
       (hs1 : supported_preservation_term t1)
       (ht2 : term_has_non_none_type t2)
       (hs2 : supported_preservation_term t2) :
-      supported_preservation_term (SmtTerm.divisible t1 t2)
+      supported_preservation_term (theory2 SmtTheoryOp.divisible t1 t2)
   | int_pow2 {t : SmtTerm}
       (ht : term_has_non_none_type t)
       (hs : supported_preservation_term t) :
-      supported_preservation_term (SmtTerm.int_pow2 t)
+      supported_preservation_term (theory1 SmtTheoryOp.int_pow2 t)
   | int_log2 {t : SmtTerm}
       (ht : term_has_non_none_type t)
       (hs : supported_preservation_term t) :
-      supported_preservation_term (SmtTerm.int_log2 t)
+      supported_preservation_term (theory1 SmtTheoryOp.int_log2 t)
   | div_total {t1 t2 : SmtTerm}
       (ht1 : term_has_non_none_type t1)
       (hs1 : supported_preservation_term t1)
       (ht2 : term_has_non_none_type t2)
       (hs2 : supported_preservation_term t2) :
-      supported_preservation_term (SmtTerm.div_total t1 t2)
+      supported_preservation_term (theory2 SmtTheoryOp.div_total t1 t2)
   | mod_total {t1 t2 : SmtTerm}
       (ht1 : term_has_non_none_type t1)
       (hs1 : supported_preservation_term t1)
       (ht2 : term_has_non_none_type t2)
       (hs2 : supported_preservation_term t2) :
-      supported_preservation_term (SmtTerm.mod_total t1 t2)
+      supported_preservation_term (theory2 SmtTheoryOp.mod_total t1 t2)
   | multmult_total {t1 t2 : SmtTerm}
       (ht1 : term_has_non_none_type t1)
       (hs1 : supported_preservation_term t1)
       (ht2 : term_has_non_none_type t2)
       (hs2 : supported_preservation_term t2) :
-      supported_preservation_term (SmtTerm.multmult_total t1 t2)
+      supported_preservation_term (theory2 SmtTheoryOp.multmult_total t1 t2)
   | qdiv {t1 t2 : SmtTerm}
       (ht1 : term_has_non_none_type t1)
       (hs1 : supported_preservation_term t1)
       (ht2 : term_has_non_none_type t2)
       (hs2 : supported_preservation_term t2) :
-      supported_preservation_term (SmtTerm.qdiv t1 t2)
+      supported_preservation_term (theory2 SmtTheoryOp.qdiv t1 t2)
   | qdiv_total {t1 t2 : SmtTerm}
       (ht1 : term_has_non_none_type t1)
       (hs1 : supported_preservation_term t1)
       (ht2 : term_has_non_none_type t2)
       (hs2 : supported_preservation_term t2) :
-      supported_preservation_term (SmtTerm.qdiv_total t1 t2)
+      supported_preservation_term (theory2 SmtTheoryOp.qdiv_total t1 t2)
   | str_len {t : SmtTerm}
       (ht : term_has_non_none_type t)
       (hs : supported_preservation_term t) :
-      supported_preservation_term (SmtTerm.str_len t)
+      supported_preservation_term (theory1 SmtTheoryOp.str_len t)
   | str_to_lower {t : SmtTerm}
       (ht : term_has_non_none_type t)
       (hs : supported_preservation_term t) :
-      supported_preservation_term (SmtTerm.str_to_lower t)
+      supported_preservation_term (theory1 SmtTheoryOp.str_to_lower t)
   | str_to_upper {t : SmtTerm}
       (ht : term_has_non_none_type t)
       (hs : supported_preservation_term t) :
-      supported_preservation_term (SmtTerm.str_to_upper t)
+      supported_preservation_term (theory1 SmtTheoryOp.str_to_upper t)
   | str_concat {t1 t2 : SmtTerm}
       (ht1 : term_has_non_none_type t1)
       (hs1 : supported_preservation_term t1)
       (ht2 : term_has_non_none_type t2)
       (hs2 : supported_preservation_term t2) :
-      supported_preservation_term (SmtTerm.str_concat t1 t2)
+      supported_preservation_term (theory2 SmtTheoryOp.str_concat t1 t2)
   | str_substr {t1 t2 t3 : SmtTerm}
       (ht1 : term_has_non_none_type t1)
       (hs1 : supported_preservation_term t1)
@@ -279,13 +279,13 @@ inductive supported_preservation_term : SmtTerm -> Prop
       (ht3 : term_has_non_none_type t3)
       (hs3 : supported_preservation_term t3) :
       supported_preservation_term
-        (SmtTerm.str_substr t1 t2 t3)
+        (theory3 SmtTheoryOp.str_substr t1 t2 t3)
   | str_contains {t1 t2 : SmtTerm}
       (ht1 : term_has_non_none_type t1)
       (hs1 : supported_preservation_term t1)
       (ht2 : term_has_non_none_type t2)
       (hs2 : supported_preservation_term t2) :
-      supported_preservation_term (SmtTerm.str_contains t1 t2)
+      supported_preservation_term (theory2 SmtTheoryOp.str_contains t1 t2)
   | str_indexof {t1 t2 t3 : SmtTerm}
       (ht1 : term_has_non_none_type t1)
       (hs1 : supported_preservation_term t1)
@@ -294,13 +294,13 @@ inductive supported_preservation_term : SmtTerm -> Prop
       (ht3 : term_has_non_none_type t3)
       (hs3 : supported_preservation_term t3) :
       supported_preservation_term
-        (SmtTerm.str_indexof t1 t2 t3)
+        (theory3 SmtTheoryOp.str_indexof t1 t2 t3)
   | str_at {t1 t2 : SmtTerm}
       (ht1 : term_has_non_none_type t1)
       (hs1 : supported_preservation_term t1)
       (ht2 : term_has_non_none_type t2)
       (hs2 : supported_preservation_term t2) :
-      supported_preservation_term (SmtTerm.str_at t1 t2)
+      supported_preservation_term (theory2 SmtTheoryOp.str_at t1 t2)
   | str_replace {t1 t2 t3 : SmtTerm}
       (ht1 : term_has_non_none_type t1)
       (hs1 : supported_preservation_term t1)
@@ -309,11 +309,11 @@ inductive supported_preservation_term : SmtTerm -> Prop
       (ht3 : term_has_non_none_type t3)
       (hs3 : supported_preservation_term t3) :
       supported_preservation_term
-        (SmtTerm.str_replace t1 t2 t3)
+        (theory3 SmtTheoryOp.str_replace t1 t2 t3)
   | str_rev {t : SmtTerm}
       (ht : term_has_non_none_type t)
       (hs : supported_preservation_term t) :
-      supported_preservation_term (SmtTerm.str_rev t)
+      supported_preservation_term (theory1 SmtTheoryOp.str_rev t)
   | str_update {t1 t2 t3 : SmtTerm}
       (ht1 : term_has_non_none_type t1)
       (hs1 : supported_preservation_term t1)
@@ -322,7 +322,7 @@ inductive supported_preservation_term : SmtTerm -> Prop
       (ht3 : term_has_non_none_type t3)
       (hs3 : supported_preservation_term t3) :
       supported_preservation_term
-        (SmtTerm.str_update t1 t2 t3)
+        (theory3 SmtTheoryOp.str_update t1 t2 t3)
   | str_replace_all {t1 t2 t3 : SmtTerm}
       (ht1 : term_has_non_none_type t1)
       (hs1 : supported_preservation_term t1)
@@ -331,7 +331,7 @@ inductive supported_preservation_term : SmtTerm -> Prop
       (ht3 : term_has_non_none_type t3)
       (hs3 : supported_preservation_term t3) :
       supported_preservation_term
-        (SmtTerm.str_replace_all t1 t2 t3)
+        (theory3 SmtTheoryOp.str_replace_all t1 t2 t3)
   | str_replace_re {t1 t2 t3 : SmtTerm}
       (ht1 : term_has_non_none_type t1)
       (hs1 : supported_preservation_term t1)
@@ -340,7 +340,7 @@ inductive supported_preservation_term : SmtTerm -> Prop
       (ht3 : term_has_non_none_type t3)
       (hs3 : supported_preservation_term t3) :
       supported_preservation_term
-        (SmtTerm.str_replace_re t1 t2 t3)
+        (theory3 SmtTheoryOp.str_replace_re t1 t2 t3)
   | str_replace_re_all {t1 t2 t3 : SmtTerm}
       (ht1 : term_has_non_none_type t1)
       (hs1 : supported_preservation_term t1)
@@ -349,7 +349,7 @@ inductive supported_preservation_term : SmtTerm -> Prop
       (ht3 : term_has_non_none_type t3)
       (hs3 : supported_preservation_term t3) :
       supported_preservation_term
-        (SmtTerm.str_replace_re_all t1 t2 t3)
+        (theory3 SmtTheoryOp.str_replace_re_all t1 t2 t3)
   | str_indexof_re {t1 t2 t3 : SmtTerm}
       (ht1 : term_has_non_none_type t1)
       (hs1 : supported_preservation_term t1)
@@ -358,122 +358,122 @@ inductive supported_preservation_term : SmtTerm -> Prop
       (ht3 : term_has_non_none_type t3)
       (hs3 : supported_preservation_term t3) :
       supported_preservation_term
-        (SmtTerm.str_indexof_re t1 t2 t3)
+        (theory3 SmtTheoryOp.str_indexof_re t1 t2 t3)
   | str_to_code {t : SmtTerm}
       (ht : term_has_non_none_type t)
       (hs : supported_preservation_term t) :
-      supported_preservation_term (SmtTerm.str_to_code t)
+      supported_preservation_term (theory1 SmtTheoryOp.str_to_code t)
   | str_to_int {t : SmtTerm}
       (ht : term_has_non_none_type t)
       (hs : supported_preservation_term t) :
-      supported_preservation_term (SmtTerm.str_to_int t)
+      supported_preservation_term (theory1 SmtTheoryOp.str_to_int t)
   | str_from_code {t : SmtTerm}
       (ht : term_has_non_none_type t)
       (hs : supported_preservation_term t) :
-      supported_preservation_term (SmtTerm.str_from_code t)
+      supported_preservation_term (theory1 SmtTheoryOp.str_from_code t)
   | str_from_int {t : SmtTerm}
       (ht : term_has_non_none_type t)
       (hs : supported_preservation_term t) :
-      supported_preservation_term (SmtTerm.str_from_int t)
+      supported_preservation_term (theory1 SmtTheoryOp.str_from_int t)
   | str_to_re {t : SmtTerm}
       (ht : term_has_non_none_type t)
       (hs : supported_preservation_term t) :
-      supported_preservation_term (SmtTerm.str_to_re t)
+      supported_preservation_term (theory1 SmtTheoryOp.str_to_re t)
   | re_mult {t : SmtTerm}
       (ht : term_has_non_none_type t)
       (hs : supported_preservation_term t) :
-      supported_preservation_term (SmtTerm.re_mult t)
+      supported_preservation_term (theory1 SmtTheoryOp.re_mult t)
   | re_plus {t : SmtTerm}
       (ht : term_has_non_none_type t)
       (hs : supported_preservation_term t) :
-      supported_preservation_term (SmtTerm.re_plus t)
+      supported_preservation_term (theory1 SmtTheoryOp.re_plus t)
   | re_exp (n : native_Int) {t : SmtTerm}
       (ht : term_has_non_none_type t)
       (hs : supported_preservation_term t) :
-      supported_preservation_term (SmtTerm.re_exp (SmtTerm.Numeral n) t)
+      supported_preservation_term (theory2 SmtTheoryOp.re_exp (SmtTerm.Numeral n) t)
   | re_opt {t : SmtTerm}
       (ht : term_has_non_none_type t)
       (hs : supported_preservation_term t) :
-      supported_preservation_term (SmtTerm.re_opt t)
+      supported_preservation_term (theory1 SmtTheoryOp.re_opt t)
   | re_comp {t : SmtTerm}
       (ht : term_has_non_none_type t)
       (hs : supported_preservation_term t) :
-      supported_preservation_term (SmtTerm.re_comp t)
+      supported_preservation_term (theory1 SmtTheoryOp.re_comp t)
   | re_range {t1 t2 : SmtTerm}
       (ht1 : term_has_non_none_type t1)
       (hs1 : supported_preservation_term t1)
       (ht2 : term_has_non_none_type t2)
       (hs2 : supported_preservation_term t2) :
-      supported_preservation_term (SmtTerm.re_range t1 t2)
+      supported_preservation_term (theory2 SmtTheoryOp.re_range t1 t2)
   | re_concat {t1 t2 : SmtTerm}
       (ht1 : term_has_non_none_type t1)
       (hs1 : supported_preservation_term t1)
       (ht2 : term_has_non_none_type t2)
       (hs2 : supported_preservation_term t2) :
-      supported_preservation_term (SmtTerm.re_concat t1 t2)
+      supported_preservation_term (theory2 SmtTheoryOp.re_concat t1 t2)
   | re_inter {t1 t2 : SmtTerm}
       (ht1 : term_has_non_none_type t1)
       (hs1 : supported_preservation_term t1)
       (ht2 : term_has_non_none_type t2)
       (hs2 : supported_preservation_term t2) :
-      supported_preservation_term (SmtTerm.re_inter t1 t2)
+      supported_preservation_term (theory2 SmtTheoryOp.re_inter t1 t2)
   | re_union {t1 t2 : SmtTerm}
       (ht1 : term_has_non_none_type t1)
       (hs1 : supported_preservation_term t1)
       (ht2 : term_has_non_none_type t2)
       (hs2 : supported_preservation_term t2) :
-      supported_preservation_term (SmtTerm.re_union t1 t2)
+      supported_preservation_term (theory2 SmtTheoryOp.re_union t1 t2)
   | re_diff {t1 t2 : SmtTerm}
       (ht1 : term_has_non_none_type t1)
       (hs1 : supported_preservation_term t1)
       (ht2 : term_has_non_none_type t2)
       (hs2 : supported_preservation_term t2) :
-      supported_preservation_term (SmtTerm.re_diff t1 t2)
+      supported_preservation_term (theory2 SmtTheoryOp.re_diff t1 t2)
   | re_loop (n1 n2 : native_Int) {t : SmtTerm}
       (ht : term_has_non_none_type t)
       (hs : supported_preservation_term t) :
       supported_preservation_term
-        (SmtTerm.re_loop (SmtTerm.Numeral n1) (SmtTerm.Numeral n2) t)
+        (theory3 SmtTheoryOp.re_loop (SmtTerm.Numeral n1) (SmtTerm.Numeral n2) t)
   | str_in_re {t1 t2 : SmtTerm}
       (ht1 : term_has_non_none_type t1)
       (hs1 : supported_preservation_term t1)
       (ht2 : term_has_non_none_type t2)
       (hs2 : supported_preservation_term t2) :
-      supported_preservation_term (SmtTerm.str_in_re t1 t2)
+      supported_preservation_term (theory2 SmtTheoryOp.str_in_re t1 t2)
   | str_lt {t1 t2 : SmtTerm}
       (ht1 : term_has_non_none_type t1)
       (hs1 : supported_preservation_term t1)
       (ht2 : term_has_non_none_type t2)
       (hs2 : supported_preservation_term t2) :
-      supported_preservation_term (SmtTerm.str_lt t1 t2)
+      supported_preservation_term (theory2 SmtTheoryOp.str_lt t1 t2)
   | str_leq {t1 t2 : SmtTerm}
       (ht1 : term_has_non_none_type t1)
       (hs1 : supported_preservation_term t1)
       (ht2 : term_has_non_none_type t2)
       (hs2 : supported_preservation_term t2) :
-      supported_preservation_term (SmtTerm.str_leq t1 t2)
+      supported_preservation_term (theory2 SmtTheoryOp.str_leq t1 t2)
   | str_prefixof {t1 t2 : SmtTerm}
       (ht1 : term_has_non_none_type t1)
       (hs1 : supported_preservation_term t1)
       (ht2 : term_has_non_none_type t2)
       (hs2 : supported_preservation_term t2) :
-      supported_preservation_term (SmtTerm.str_prefixof t1 t2)
+      supported_preservation_term (theory2 SmtTheoryOp.str_prefixof t1 t2)
   | str_suffixof {t1 t2 : SmtTerm}
       (ht1 : term_has_non_none_type t1)
       (hs1 : supported_preservation_term t1)
       (ht2 : term_has_non_none_type t2)
       (hs2 : supported_preservation_term t2) :
-      supported_preservation_term (SmtTerm.str_suffixof t1 t2)
+      supported_preservation_term (theory2 SmtTheoryOp.str_suffixof t1 t2)
   | str_is_digit {t : SmtTerm}
       (ht : term_has_non_none_type t)
       (hs : supported_preservation_term t) :
-      supported_preservation_term (SmtTerm.str_is_digit t)
+      supported_preservation_term (theory1 SmtTheoryOp.str_is_digit t)
   | bv_concat {t1 t2 : SmtTerm}
       (ht1 : term_has_non_none_type t1)
       (hs1 : supported_preservation_term t1)
       (ht2 : term_has_non_none_type t2)
       (hs2 : supported_preservation_term t2) :
-      supported_preservation_term (SmtTerm.concat t1 t2)
+      supported_preservation_term (theory2 SmtTheoryOp.concat t1 t2)
   | extract {t1 t2 t3 : SmtTerm}
       (ht1 : term_has_non_none_type t1)
       (hs1 : supported_preservation_term t1)
@@ -482,261 +482,261 @@ inductive supported_preservation_term : SmtTerm -> Prop
       (ht3 : term_has_non_none_type t3)
       (hs3 : supported_preservation_term t3) :
       supported_preservation_term
-        (SmtTerm.extract t1 t2 t3)
+        (theory3 SmtTheoryOp.extract t1 t2 t3)
   | bvnot {t : SmtTerm}
       (ht : term_has_non_none_type t)
       (hs : supported_preservation_term t) :
-      supported_preservation_term (SmtTerm.bvnot t)
+      supported_preservation_term (theory1 SmtTheoryOp.bvnot t)
   | bvand {t1 t2 : SmtTerm}
       (ht1 : term_has_non_none_type t1)
       (hs1 : supported_preservation_term t1)
       (ht2 : term_has_non_none_type t2)
       (hs2 : supported_preservation_term t2) :
-      supported_preservation_term (SmtTerm.bvand t1 t2)
+      supported_preservation_term (theory2 SmtTheoryOp.bvand t1 t2)
   | bvor {t1 t2 : SmtTerm}
       (ht1 : term_has_non_none_type t1)
       (hs1 : supported_preservation_term t1)
       (ht2 : term_has_non_none_type t2)
       (hs2 : supported_preservation_term t2) :
-      supported_preservation_term (SmtTerm.bvor t1 t2)
+      supported_preservation_term (theory2 SmtTheoryOp.bvor t1 t2)
   | bvnand {t1 t2 : SmtTerm}
       (ht1 : term_has_non_none_type t1)
       (hs1 : supported_preservation_term t1)
       (ht2 : term_has_non_none_type t2)
       (hs2 : supported_preservation_term t2) :
-      supported_preservation_term (SmtTerm.bvnand t1 t2)
+      supported_preservation_term (theory2 SmtTheoryOp.bvnand t1 t2)
   | bvnor {t1 t2 : SmtTerm}
       (ht1 : term_has_non_none_type t1)
       (hs1 : supported_preservation_term t1)
       (ht2 : term_has_non_none_type t2)
       (hs2 : supported_preservation_term t2) :
-      supported_preservation_term (SmtTerm.bvnor t1 t2)
+      supported_preservation_term (theory2 SmtTheoryOp.bvnor t1 t2)
   | bvxor {t1 t2 : SmtTerm}
       (ht1 : term_has_non_none_type t1)
       (hs1 : supported_preservation_term t1)
       (ht2 : term_has_non_none_type t2)
       (hs2 : supported_preservation_term t2) :
-      supported_preservation_term (SmtTerm.bvxor t1 t2)
+      supported_preservation_term (theory2 SmtTheoryOp.bvxor t1 t2)
   | bvxnor {t1 t2 : SmtTerm}
       (ht1 : term_has_non_none_type t1)
       (hs1 : supported_preservation_term t1)
       (ht2 : term_has_non_none_type t2)
       (hs2 : supported_preservation_term t2) :
-      supported_preservation_term (SmtTerm.bvxnor t1 t2)
+      supported_preservation_term (theory2 SmtTheoryOp.bvxnor t1 t2)
   | bvcomp {t1 t2 : SmtTerm}
       (ht1 : term_has_non_none_type t1)
       (hs1 : supported_preservation_term t1)
       (ht2 : term_has_non_none_type t2)
       (hs2 : supported_preservation_term t2) :
-      supported_preservation_term (SmtTerm.bvcomp t1 t2)
+      supported_preservation_term (theory2 SmtTheoryOp.bvcomp t1 t2)
   | bvneg {t : SmtTerm}
       (ht : term_has_non_none_type t)
       (hs : supported_preservation_term t) :
-      supported_preservation_term (SmtTerm.bvneg t)
+      supported_preservation_term (theory1 SmtTheoryOp.bvneg t)
   | bvadd {t1 t2 : SmtTerm}
       (ht1 : term_has_non_none_type t1)
       (hs1 : supported_preservation_term t1)
       (ht2 : term_has_non_none_type t2)
       (hs2 : supported_preservation_term t2) :
-      supported_preservation_term (SmtTerm.bvadd t1 t2)
+      supported_preservation_term (theory2 SmtTheoryOp.bvadd t1 t2)
   | bvmul {t1 t2 : SmtTerm}
       (ht1 : term_has_non_none_type t1)
       (hs1 : supported_preservation_term t1)
       (ht2 : term_has_non_none_type t2)
       (hs2 : supported_preservation_term t2) :
-      supported_preservation_term (SmtTerm.bvmul t1 t2)
+      supported_preservation_term (theory2 SmtTheoryOp.bvmul t1 t2)
   | bvudiv {t1 t2 : SmtTerm}
       (ht1 : term_has_non_none_type t1)
       (hs1 : supported_preservation_term t1)
       (ht2 : term_has_non_none_type t2)
       (hs2 : supported_preservation_term t2) :
-      supported_preservation_term (SmtTerm.bvudiv t1 t2)
+      supported_preservation_term (theory2 SmtTheoryOp.bvudiv t1 t2)
   | bvurem {t1 t2 : SmtTerm}
       (ht1 : term_has_non_none_type t1)
       (hs1 : supported_preservation_term t1)
       (ht2 : term_has_non_none_type t2)
       (hs2 : supported_preservation_term t2) :
-      supported_preservation_term (SmtTerm.bvurem t1 t2)
+      supported_preservation_term (theory2 SmtTheoryOp.bvurem t1 t2)
   | bvsub {t1 t2 : SmtTerm}
       (ht1 : term_has_non_none_type t1)
       (hs1 : supported_preservation_term t1)
       (ht2 : term_has_non_none_type t2)
       (hs2 : supported_preservation_term t2) :
-      supported_preservation_term (SmtTerm.bvsub t1 t2)
+      supported_preservation_term (theory2 SmtTheoryOp.bvsub t1 t2)
   | bvult {t1 t2 : SmtTerm}
       (ht1 : term_has_non_none_type t1)
       (hs1 : supported_preservation_term t1)
       (ht2 : term_has_non_none_type t2)
       (hs2 : supported_preservation_term t2) :
-      supported_preservation_term (SmtTerm.bvult t1 t2)
+      supported_preservation_term (theory2 SmtTheoryOp.bvult t1 t2)
   | bvule {t1 t2 : SmtTerm}
       (ht1 : term_has_non_none_type t1)
       (hs1 : supported_preservation_term t1)
       (ht2 : term_has_non_none_type t2)
       (hs2 : supported_preservation_term t2) :
-      supported_preservation_term (SmtTerm.bvule t1 t2)
+      supported_preservation_term (theory2 SmtTheoryOp.bvule t1 t2)
   | bvugt {t1 t2 : SmtTerm}
       (ht1 : term_has_non_none_type t1)
       (hs1 : supported_preservation_term t1)
       (ht2 : term_has_non_none_type t2)
       (hs2 : supported_preservation_term t2) :
-      supported_preservation_term (SmtTerm.bvugt t1 t2)
+      supported_preservation_term (theory2 SmtTheoryOp.bvugt t1 t2)
   | bvuge {t1 t2 : SmtTerm}
       (ht1 : term_has_non_none_type t1)
       (hs1 : supported_preservation_term t1)
       (ht2 : term_has_non_none_type t2)
       (hs2 : supported_preservation_term t2) :
-      supported_preservation_term (SmtTerm.bvuge t1 t2)
+      supported_preservation_term (theory2 SmtTheoryOp.bvuge t1 t2)
   | bvslt {t1 t2 : SmtTerm}
       (ht1 : term_has_non_none_type t1)
       (hs1 : supported_preservation_term t1)
       (ht2 : term_has_non_none_type t2)
       (hs2 : supported_preservation_term t2) :
-      supported_preservation_term (SmtTerm.bvslt t1 t2)
+      supported_preservation_term (theory2 SmtTheoryOp.bvslt t1 t2)
   | bvsle {t1 t2 : SmtTerm}
       (ht1 : term_has_non_none_type t1)
       (hs1 : supported_preservation_term t1)
       (ht2 : term_has_non_none_type t2)
       (hs2 : supported_preservation_term t2) :
-      supported_preservation_term (SmtTerm.bvsle t1 t2)
+      supported_preservation_term (theory2 SmtTheoryOp.bvsle t1 t2)
   | bvsgt {t1 t2 : SmtTerm}
       (ht1 : term_has_non_none_type t1)
       (hs1 : supported_preservation_term t1)
       (ht2 : term_has_non_none_type t2)
       (hs2 : supported_preservation_term t2) :
-      supported_preservation_term (SmtTerm.bvsgt t1 t2)
+      supported_preservation_term (theory2 SmtTheoryOp.bvsgt t1 t2)
   | bvsge {t1 t2 : SmtTerm}
       (ht1 : term_has_non_none_type t1)
       (hs1 : supported_preservation_term t1)
       (ht2 : term_has_non_none_type t2)
       (hs2 : supported_preservation_term t2) :
-      supported_preservation_term (SmtTerm.bvsge t1 t2)
+      supported_preservation_term (theory2 SmtTheoryOp.bvsge t1 t2)
   | bvshl {t1 t2 : SmtTerm}
       (ht1 : term_has_non_none_type t1)
       (hs1 : supported_preservation_term t1)
       (ht2 : term_has_non_none_type t2)
       (hs2 : supported_preservation_term t2) :
-      supported_preservation_term (SmtTerm.bvshl t1 t2)
+      supported_preservation_term (theory2 SmtTheoryOp.bvshl t1 t2)
   | bvlshr {t1 t2 : SmtTerm}
       (ht1 : term_has_non_none_type t1)
       (hs1 : supported_preservation_term t1)
       (ht2 : term_has_non_none_type t2)
       (hs2 : supported_preservation_term t2) :
-      supported_preservation_term (SmtTerm.bvlshr t1 t2)
+      supported_preservation_term (theory2 SmtTheoryOp.bvlshr t1 t2)
   | repeat {t1 t2 : SmtTerm}
       (ht1 : term_has_non_none_type t1)
       (hs1 : supported_preservation_term t1)
       (ht2 : term_has_non_none_type t2)
       (hs2 : supported_preservation_term t2) :
-      supported_preservation_term (SmtTerm.repeat t1 t2)
+      supported_preservation_term (theory2 SmtTheoryOp.repeat t1 t2)
   | bvsdiv {t1 t2 : SmtTerm}
       (ht1 : term_has_non_none_type t1)
       (hs1 : supported_preservation_term t1)
       (ht2 : term_has_non_none_type t2)
       (hs2 : supported_preservation_term t2) :
-      supported_preservation_term (SmtTerm.bvsdiv t1 t2)
+      supported_preservation_term (theory2 SmtTheoryOp.bvsdiv t1 t2)
   | bvsrem {t1 t2 : SmtTerm}
       (ht1 : term_has_non_none_type t1)
       (hs1 : supported_preservation_term t1)
       (ht2 : term_has_non_none_type t2)
       (hs2 : supported_preservation_term t2) :
-      supported_preservation_term (SmtTerm.bvsrem t1 t2)
+      supported_preservation_term (theory2 SmtTheoryOp.bvsrem t1 t2)
   | bvsmod {t1 t2 : SmtTerm}
       (ht1 : term_has_non_none_type t1)
       (hs1 : supported_preservation_term t1)
       (ht2 : term_has_non_none_type t2)
       (hs2 : supported_preservation_term t2) :
-      supported_preservation_term (SmtTerm.bvsmod t1 t2)
+      supported_preservation_term (theory2 SmtTheoryOp.bvsmod t1 t2)
   | bvashr {t1 t2 : SmtTerm}
       (ht1 : term_has_non_none_type t1)
       (hs1 : supported_preservation_term t1)
       (ht2 : term_has_non_none_type t2)
       (hs2 : supported_preservation_term t2) :
-      supported_preservation_term (SmtTerm.bvashr t1 t2)
+      supported_preservation_term (theory2 SmtTheoryOp.bvashr t1 t2)
   | rotate_left {t1 t2 : SmtTerm}
       (ht1 : term_has_non_none_type t1)
       (hs1 : supported_preservation_term t1)
       (ht2 : term_has_non_none_type t2)
       (hs2 : supported_preservation_term t2) :
-      supported_preservation_term (SmtTerm.rotate_left t1 t2)
+      supported_preservation_term (theory2 SmtTheoryOp.rotate_left t1 t2)
   | rotate_right {t1 t2 : SmtTerm}
       (ht1 : term_has_non_none_type t1)
       (hs1 : supported_preservation_term t1)
       (ht2 : term_has_non_none_type t2)
       (hs2 : supported_preservation_term t2) :
-      supported_preservation_term (SmtTerm.rotate_right t1 t2)
+      supported_preservation_term (theory2 SmtTheoryOp.rotate_right t1 t2)
   | bvuaddo {t1 t2 : SmtTerm}
       (ht1 : term_has_non_none_type t1)
       (hs1 : supported_preservation_term t1)
       (ht2 : term_has_non_none_type t2)
       (hs2 : supported_preservation_term t2) :
-      supported_preservation_term (SmtTerm.bvuaddo t1 t2)
+      supported_preservation_term (theory2 SmtTheoryOp.bvuaddo t1 t2)
   | bvnego {t : SmtTerm}
       (ht : term_has_non_none_type t)
       (hs : supported_preservation_term t) :
-      supported_preservation_term (SmtTerm.bvnego t)
+      supported_preservation_term (theory1 SmtTheoryOp.bvnego t)
   | bvsaddo {t1 t2 : SmtTerm}
       (ht1 : term_has_non_none_type t1)
       (hs1 : supported_preservation_term t1)
       (ht2 : term_has_non_none_type t2)
       (hs2 : supported_preservation_term t2) :
-      supported_preservation_term (SmtTerm.bvsaddo t1 t2)
+      supported_preservation_term (theory2 SmtTheoryOp.bvsaddo t1 t2)
   | bvumulo {t1 t2 : SmtTerm}
       (ht1 : term_has_non_none_type t1)
       (hs1 : supported_preservation_term t1)
       (ht2 : term_has_non_none_type t2)
       (hs2 : supported_preservation_term t2) :
-      supported_preservation_term (SmtTerm.bvumulo t1 t2)
+      supported_preservation_term (theory2 SmtTheoryOp.bvumulo t1 t2)
   | bvsmulo {t1 t2 : SmtTerm}
       (ht1 : term_has_non_none_type t1)
       (hs1 : supported_preservation_term t1)
       (ht2 : term_has_non_none_type t2)
       (hs2 : supported_preservation_term t2) :
-      supported_preservation_term (SmtTerm.bvsmulo t1 t2)
+      supported_preservation_term (theory2 SmtTheoryOp.bvsmulo t1 t2)
   | bvusubo {t1 t2 : SmtTerm}
       (ht1 : term_has_non_none_type t1)
       (hs1 : supported_preservation_term t1)
       (ht2 : term_has_non_none_type t2)
       (hs2 : supported_preservation_term t2) :
-      supported_preservation_term (SmtTerm.bvusubo t1 t2)
+      supported_preservation_term (theory2 SmtTheoryOp.bvusubo t1 t2)
   | bvssubo {t1 t2 : SmtTerm}
       (ht1 : term_has_non_none_type t1)
       (hs1 : supported_preservation_term t1)
       (ht2 : term_has_non_none_type t2)
       (hs2 : supported_preservation_term t2) :
-      supported_preservation_term (SmtTerm.bvssubo t1 t2)
+      supported_preservation_term (theory2 SmtTheoryOp.bvssubo t1 t2)
   | bvsdivo {t1 t2 : SmtTerm}
       (ht1 : term_has_non_none_type t1)
       (hs1 : supported_preservation_term t1)
       (ht2 : term_has_non_none_type t2)
       (hs2 : supported_preservation_term t2) :
-      supported_preservation_term (SmtTerm.bvsdivo t1 t2)
+      supported_preservation_term (theory2 SmtTheoryOp.bvsdivo t1 t2)
   | zero_extend {t1 t2 : SmtTerm}
       (ht1 : term_has_non_none_type t1)
       (hs1 : supported_preservation_term t1)
       (ht2 : term_has_non_none_type t2)
       (hs2 : supported_preservation_term t2) :
-      supported_preservation_term (SmtTerm.zero_extend t1 t2)
+      supported_preservation_term (theory2 SmtTheoryOp.zero_extend t1 t2)
   | sign_extend {t1 t2 : SmtTerm}
       (ht1 : term_has_non_none_type t1)
       (hs1 : supported_preservation_term t1)
       (ht2 : term_has_non_none_type t2)
       (hs2 : supported_preservation_term t2) :
-      supported_preservation_term (SmtTerm.sign_extend t1 t2)
+      supported_preservation_term (theory2 SmtTheoryOp.sign_extend t1 t2)
   | int_to_bv {t1 t2 : SmtTerm}
       (ht1 : term_has_non_none_type t1)
       (hs1 : supported_preservation_term t1)
       (ht2 : term_has_non_none_type t2)
       (hs2 : supported_preservation_term t2) :
-      supported_preservation_term (SmtTerm.int_to_bv t1 t2)
+      supported_preservation_term (theory2 SmtTheoryOp.int_to_bv t1 t2)
   | ubv_to_int {t : SmtTerm}
       (ht : term_has_non_none_type t)
       (hs : supported_preservation_term t) :
-      supported_preservation_term (SmtTerm.ubv_to_int t)
+      supported_preservation_term (theory1 SmtTheoryOp.ubv_to_int t)
   | sbv_to_int {t : SmtTerm}
       (ht : term_has_non_none_type t)
       (hs : supported_preservation_term t) :
-      supported_preservation_term (SmtTerm.sbv_to_int t)
+      supported_preservation_term (theory1 SmtTheoryOp.sbv_to_int t)
   | dt_cons (s : native_String) (d : SmtDatatype) (i : native_Nat) :
       supported_preservation_term (SmtTerm.DtCons s d i)
   | dt_sel {s : native_String} {d : SmtDatatype} {i j : native_Nat} {x : SmtTerm}
